More erasure

template-coq/theories/Erasure/Ast.v
@@ -32,3 +32,185 @@ Inductive term : Set :=
 | tProj      : projection -> term -> term
 | tFix       : mfixpoint term -> nat -> term
 | tCoFix     : mfixpoint term -> nat -> term.
+
+
+
+Definition mkApps t us :=
+  match us with
+  | nil => t
+  | _ => match t with
+        | tApp f args => tApp f (args ++ us)
+        | _ => tApp t us
+        end
+  end.
+
+Definition mkApp t u := Eval cbn in mkApps t [u].
+
+Definition isApp t :=
+  match t with
+  | tApp _ _ => true
+  | _ => false
+  end.
+
+(** Well-formed terms: invariants which are not ensured by the OCaml type system *)
+
+Inductive wf : term -> Prop :=
+| wf_tBox : wf tBox
+| wf_tRel n : wf (tRel n)
+| wf_tVar id : wf (tVar id)
+| wf_tMeta n : wf (tMeta n)
+| wf_tEvar n l : Forall wf l -> wf (tEvar n l)
+| wf_tSort u : wf (tSort u)
+| wf_tProd na t b : wf t -> wf b -> wf (tProd na t b)
+| wf_tLambda na t b : wf t -> wf b -> wf (tLambda na t b)
+| wf_tLetIn na t b b' : wf t -> wf b -> wf b' -> wf (tLetIn na t b b')
+| wf_tApp t u : ~ isApp t = true -> u <> nil -> wf t -> Forall wf u -> wf (tApp t u)
+| wf_tConst k u : wf (tConst k u)
+| wf_tInd i u : wf (tInd i u)
+| wf_tConstruct i k u : wf (tConstruct i k u)
+| wf_tCase ci p c brs : wf p -> wf c -> Forall (Program.Basics.compose wf snd) brs -> wf (tCase ci p c brs)
+| wf_tProj p t : wf t -> wf (tProj p t)
+| wf_tFix mfix k : Forall (fun def => wf def.(dtype _) /\ wf def.(dbody _)) mfix -> wf (tFix mfix k)
+| wf_tCoFix mfix k : Forall (fun def => wf def.(dtype _) /\ wf def.(dbody _)) mfix -> wf (tCoFix mfix k).
+
+(** ** Entries
+
+  The kernel accepts these inputs and typechecks them to produce
+  declarations. Reflects [kernel/entries.mli].
+*)
+
+(** *** Constant and axiom entries *)
+
+Record parameter_entry := {
+  parameter_entry_type      : term;
+  parameter_entry_universes : universe_context }.
+
+Record definition_entry := {
+  definition_entry_type      : term;
+  definition_entry_body      : term;
+  definition_entry_universes : universe_context;
+  definition_entry_opaque    : bool }.
+
+
+Inductive constant_entry :=
+| ParameterEntry  (p : parameter_entry)
+| DefinitionEntry (def : definition_entry).
+
+(** *** Inductive entries *)
+
+(** This is the representation of mutual inductives.
+    nearly copied from [kernel/entries.mli]
+
+  Assume the following definition in concrete syntax:
+
+[[
+  Inductive I1 (x1:X1) ... (xn:Xn) : A1 := c11 : T11 | ... | c1n1 : T1n1
+  ...
+  with      Ip (x1:X1) ... (xn:Xn) : Ap := cp1 : Tp1  ... | cpnp : Tpnp.
+]]
+
+  then, in [i]th block, [mind_entry_params] is [xn:Xn;...;x1:X1];
+  [mind_entry_arity] is [Ai], defined in context [x1:X1;...;xn:Xn];
+  [mind_entry_lc] is [Ti1;...;Tini], defined in context
+  [A'1;...;A'p;x1:X1;...;xn:Xn] where [A'i] is [Ai] generalized over
+  [x1:X1;...;xn:Xn].
+*)
+
+Inductive recursivity_kind :=
+  | Finite (* = inductive *)
+  | CoFinite (* = coinductive *)
+  | BiFinite (* = non-recursive, like in "Record" definitions *).
+
+Inductive local_entry : Set :=
+| LocalDef : term -> local_entry (* local let binding *)
+| LocalAssum : term -> local_entry.
+
+Record one_inductive_entry : Set := {
+  mind_entry_typename : ident;
+  mind_entry_arity : term;
+  mind_entry_template : bool; (* template polymorphism *)
+  mind_entry_consnames : list ident;
+  mind_entry_lc : list term (* constructor list *) }.
+
+Record mutual_inductive_entry := {
+  mind_entry_record    : option (option ident);
+  (* Is this mutual inductive defined as a record?
+     If so, is it primitive, using binder name [ident]
+     for the record in primitive projections ? *)
+  mind_entry_finite    : recursivity_kind;
+  mind_entry_params    : list (ident * local_entry);
+  mind_entry_inds      : list one_inductive_entry;
+  mind_entry_universes : universe_context;
+  mind_entry_private   : option bool
+  (* Private flag for sealing an inductive definition in an enclosing
+     module. Not handled by Template Coq yet. *) }.
+
+
+
+(** ** Declarations *)
+
+(** *** The context of De Bruijn indices *)
+
+Record context_decl := {
+  decl_name : name ;
+  decl_body : option term ;
+  decl_type : term }.
+
+(** Local (de Bruijn) variable binding *)
+
+Definition vass x A := {| decl_name := x; decl_body := None; decl_type := A |}.
+
+(** Local (de Bruijn) let-binding *)
+
+Definition vdef x t A := {| decl_name := x; decl_body := Some t; decl_type := A |}.
+
+(** Local (de Bruijn) context *)
+
+Definition context := list context_decl.
+
+(** Last declaration first *)
+
+Definition snoc {A} (Γ : list A) (d : A) := d :: Γ.
+
+Notation " Γ ,, d " := (snoc Γ d) (at level 20, d at next level).
+
+(** *** Environments *)
+
+(** See [one_inductive_body] from [declarations.ml]. *)
+Record one_inductive_body := {
+  ind_name : ident;
+  ind_type : term; (* Closed arity *)
+  ind_kelim : list sort_family; (* Allowed elimination sorts *)
+  ind_ctors : list (ident * term (* Under context of arities of the mutual inductive *)
+                    * nat (* arity, w/o lets, w/o parameters *));
+  ind_projs : list (ident * term) (* names and types of projections, if any.
+                                     Type under context of params and inductive object *) }.
+
+(** See [mutual_inductive_body] from [declarations.ml]. *)
+Record mutual_inductive_body := {
+  ind_npars : nat;
+  ind_bodies : list one_inductive_body ;
+  ind_universes : universe_context }.
+
+(** See [constant_body] from [declarations.ml] *)
+Record constant_body := {
+    cst_type : term;
+    cst_body : option term;
+    cst_universes : universe_context }.
+
+Inductive global_decl :=
+| ConstantDecl : kername -> constant_body -> global_decl
+| InductiveDecl : kername -> mutual_inductive_body -> global_decl.
+
+Definition global_declarations := list global_decl.
+
+(** A context of global declarations + global universe constraints,
+    i.e. a global environment *)
+
+Definition global_context : Type := global_declarations * uGraph.t.
+
+(** *** Programs
+
+  A set of declarations and a term, as produced by [Quote Recursively]. *)
+
+Definition program : Type := global_declarations * term.
