template-coq/theories/Erasure/LiftSubst.v
@@ -1,0 +1,527 @@
+(* Distributed under the terms of the MIT license.   *)
+
+Require Import List Program.
+Require Import Erasure.Ast.
+Require Import BinPos.
+Require Import Coq.Arith.Compare_dec Bool.
+Require Import Erasure.Induction.
+
+(** * Lifting and substitution for the AST
+
+  Along with standard commutation lemmas.
+  Definition of [closedn] (boolean) predicate for checking if
+  a term is closed. *)
+
+Set Asymmetric Patterns.
+
+Fixpoint lift n k t : term :=
+  match t with
+  | tRel i => if Nat.leb k i then tRel (n + i) else tRel i
+  | tEvar ev args => tEvar ev (List.map (lift n k) args)
+  | tLambda na T M => tLambda na (lift n k T) (lift n (S k) M)
+  | tApp u v => tApp (lift n k u) (List.map (lift n k) v)
+  | tProd na A B => tProd na (lift n k A) (lift n (S k) B)
+  | tLetIn na b t b' => tLetIn na (lift n k b) (lift n k t) (lift n (S k) b')
+  | tCase ind p c brs =>
+    let brs' := List.map (on_snd (lift n k)) brs in
+    tCase ind (lift n k p) (lift n k c) brs'
+  | tProj p c => tProj p (lift n k c)
+  | tFix mfix idx =>
+    let k' := List.length mfix + k in
+    let mfix' := List.map (map_def (lift n k')) mfix in
+    tFix mfix' idx
+  | tCoFix mfix idx =>
+    let k' := List.length mfix + k in
+    let mfix' := List.map (map_def (lift n k')) mfix in
+    tCoFix mfix' idx
+  | x => x
+  end.
+
+
+Notation lift0 n := (lift n 0).
+Definition up := lift 1 0.
+
+Fixpoint subst t k u :=
+  match u with
+  | tRel n =>
+    match Nat.compare k n with
+    | Datatypes.Eq => lift0 k t
+    | Datatypes.Gt => tRel n
+    | Datatypes.Lt => tRel (pred n)
+    end
+  | tEvar ev args => tEvar ev (List.map (subst t k) args)
+  | tLambda na T M => tLambda na (subst t k T) (subst t (S k) M)
+  | tApp u v => mkApps (subst t k u) (List.map (subst t k) v)
+  | tProd na A B => tProd na (subst t k A) (subst t (S k) B)
+  | tLetIn na b ty b' => tLetIn na (subst t k b) (subst t k ty) (subst t (S k) b')
+  | tCase ind p c brs =>
+    let brs' := List.map (on_snd (subst t k)) brs in
+    tCase ind (subst t k p) (subst t k c) brs'
+  | tProj p c => tProj p (subst t k c)
+  | tFix mfix idx =>
+    let k' := List.length mfix + k in
+    let mfix' := List.map (map_def (subst t k')) mfix in
+    tFix mfix' idx
+  | tCoFix mfix idx =>
+    let k' := List.length mfix + k in
+    let mfix' := List.map (map_def (subst t k')) mfix in
+    tCoFix mfix' idx
+  | x => x
+  end.
+
+Notation subst0 t := (subst t 0).
+Notation "M { j := N }" := (subst N j M) (at level 10, right associativity).
+
+(** Substitutes [t1 ; .. ; tn] in u for [Rel 0; .. Rel (n-1)]*)
+Definition substl l t :=
+  List.fold_left (fun t u => subst0 u t) l t.
+
+Fixpoint closedn k (t : term) : bool :=
+  match t with
+  | tRel i => Nat.ltb i k
+  | tEvar ev args => List.forallb (closedn k) args
+  | tLambda _ T M | tProd _ T M => closedn k T && closedn (S k) M
+  | tApp u v => closedn k u && List.forallb (closedn k) v
+  | tLetIn na b t b' => closedn k b && closedn k t && closedn (S k) b'
+  | tCase ind p c brs =>
+    let brs' := List.forallb (test_snd (closedn k)) brs in
+    closedn k p && closedn k c && brs'
+  | tProj p c => closedn k c
+  | tFix mfix idx =>
+    let k' := List.length mfix + k in
+    List.forallb (test_def (closedn k')) mfix
+  | tCoFix mfix idx =>
+    let k' := List.length mfix + k in
+    List.forallb (test_def (closedn k')) mfix
+  | x => true
+  end.
+
+Notation closed t := (closedn 0 t).
+
+Create HintDb terms.
+
+Ltac easy0 :=
+  let rec use_hyp H :=
+   (match type of H with
+    | _ /\ _ => exact H || destruct_hyp H
+    | _ => try (solve [ inversion H ])
+    end)
+  with do_intro := (let H := fresh in
+                    intro H; use_hyp H)
+  with destruct_hyp H := (case H; clear H; do_intro; do_intro)
+  in
+  let rec use_hyps :=
+   (match goal with
+    | H:_ /\ _ |- _ => exact H || (destruct_hyp H; use_hyps)
+    | H:_ |- _ => solve [ inversion H ]
+    | _ => idtac
+    end)
+  in
+  let do_atom := (solve [ trivial with eq_true | reflexivity | symmetry; trivial | contradiction ]) in
+  let rec do_ccl := (try do_atom; repeat (do_intro; try do_atom); (solve [ split; do_ccl ])) in
+  (solve [ do_atom | use_hyps; do_ccl ]) || fail "Cannot solve this goal".
+Require Import Omega.
+Hint Extern 100 => omega : terms.
+
+Ltac easy ::= easy0 || solve [eauto 7 with core arith terms].
+
+Notation lift_rec n c k := (lift n k c) (only parsing).
+Notation subst_rec N M k := (subst N k M) (only parsing).
+
+Require Import PeanoNat.
+Import Nat.
+
+Lemma lift_rel_ge :
+  forall k n p, p <= n -> lift_rec k (tRel n) p = tRel (k + n).
+Proof.
+  intros; simpl in |- *.
+  now elim (leb_spec p n).
+Qed.
+
+Lemma lift_rel_lt : forall k n p, p > n -> lift_rec k (tRel n) p = tRel n.
+Proof.
+  intros; simpl in |- *.
+  now elim (leb_spec p n).
+Qed.
+
+Lemma lift_rel_alt : forall n k i, lift n k (tRel i) = tRel (if Nat.leb k i then n + i else i).
+Proof.
+  intros; simpl. now destruct leb.
+Qed.
+
+Lemma subst_rel_lt : forall u n k, k > n -> subst_rec u (tRel n) k = tRel n.
+Proof.
+  simpl in |- *; intros.
+  elim (compare_spec k n); intro Hcomp; easy.
+Qed.
+
+Lemma subst_rel_gt :
+  forall u n k, n > k -> subst_rec u (tRel n) k = tRel (pred n).
+Proof.
+  simpl in |- *; intros.
+  now elim (compare_spec k n). 
+Qed.
+
+Lemma subst_rel_eq : forall u n, subst_rec u (tRel n) n = lift0 n u.
+Proof.
+  intros; simpl in |- *.
+  now elim (compare_spec n n).
+Qed.
+
+Lemma lift_rec0 : forall M k, lift_rec 0 M k = M.
+Proof.
+  intros M.
+  elim M using term_forall_list_ind; simpl in |- *; intros; try easy ;
+    try (try rewrite H; try rewrite H0 ; try rewrite H1 ; easy).
+
+  - now elim (leb k n).
+  - f_equal. rewrite <- map_id. now eapply (forall_map_spec H).
+  - f_equal. auto. rewrite <- map_id. now eapply (forall_map_spec H0).
+  - f_equal; auto. rewrite <- map_id. eapply (forall_map_spec H1).
+    intros. destruct x; unfold on_snd. simpl. rewrite H2. reflexivity.
+
+  - f_equal. transitivity (map (map_def id) m). eapply (tfix_map_spec H); auto.
+    rewrite <- map_id. f_equal. extensionality x. destruct x; reflexivity.
+  - f_equal. transitivity (map (map_def id) m). eapply (tfix_map_spec H); auto.
+    rewrite <- map_id. f_equal. extensionality x. destruct x; reflexivity.
+Qed.
+
+Lemma lift0_p : forall M, lift0 0 M = M.
+  intros; unfold lift in |- *.
+  apply lift_rec0; easy.
+Qed.
+
+
+Lemma simpl_lift_rec :
+  forall M n k p i,
+    i <= k + n ->
+    k <= i -> lift_rec p (lift_rec n M k) i = lift_rec (p + n) M k.
+Proof.
+  intros M.
+  elim M using term_forall_list_ind;
+    intros; simpl; try easy;
+      rewrite ?map_map_compose, ?compose_on_snd, ?compose_map_def;
+      try (rewrite H, ?H0, ?H1; auto); try (f_equal; apply_spec);
+        try rewrite ?map_length; try easy.
+
+  - elim (leb_spec k n); intros.
+    now rewrite lift_rel_ge.
+    now rewrite lift_rel_lt.
+Qed.
+
+Lemma simpl_lift : forall M n, lift0 (S n) M = lift0 1 (lift0 n M).
+  now intros; rewrite simpl_lift_rec.
+Qed.
+
+Lemma permute_lift_rec :
+  forall M n k p i,
+    i <= k ->
+    lift_rec p (lift_rec n M k) i = lift_rec n (lift_rec p M i) (p + k).
+Proof.
+  intros M.
+  elim M using term_forall_list_ind;
+    intros; simpl; try easy;
+      rewrite ?map_map_compose, ?compose_on_snd, ?compose_map_def;
+      try solve [f_equal; easy];
+      try (f_equal; try easy; apply_spec);
+      unfold compose; intros;
+        try rewrite ?map_length; try easy ;
+        try (rewrite H, H0; f_equal; try easy; now f_equal);
+        try (rewrite H, H0, H1; f_equal; try easy; now f_equal);
+        try (rewrite H1; now f_equal).
+  
+  - elim (leb_spec k n); intros;
+    elim (leb_spec i n); intros; try easy.
+    + rewrite 2!lift_rel_ge; try easy.
+    + rewrite lift_rel_ge, lift_rel_lt; try easy.
+    + rewrite 2!lift_rel_lt; try easy.
+Qed.
+
+Lemma permute_lift :
+  forall M k, lift0 1 (lift_rec 1 M k) = lift_rec 1 (lift0 1 M) (S k).
+  intros.
+  change (lift_rec 1 (lift_rec 1 M k) 0 = lift_rec 1 (lift_rec 1 M 0) (1 + k))
+    in |- *.
+  apply permute_lift_rec; easy.
+Qed.
+
+Lemma Forall_map {A B} (P : B -> Prop) (f : A -> B) l : Forall (Program.Basics.compose P f) l -> Forall P (map f l).
+Proof.
+  induction 1; constructor; auto.
+Qed.
+
+Lemma Forall_impl {A} (P Q : A -> Prop) : forall l, Forall P l -> (forall x, P x -> Q x) -> Forall Q l.
+Proof.
+  induction 1; constructor; auto.
+Qed.
+
+Lemma lift_rec_isApp n k t : ~ isApp t = true -> ~ isApp (lift n k t) = true.
+Proof.
+  induction t; auto.
+  intros.
+  simpl. destruct leb; auto.
+Qed.
+
+Lemma map_non_nil {A B} (f : A -> B) l : l <> nil -> map f l <> nil.
+Proof.
+  intros. intro.
+  destruct l; try discriminate.
+  contradiction.
+Qed.
+
+Lemma lift_rec_wf n k t : wf t -> wf (lift_rec n t k).
+Proof.
+  intros wft; revert t wft k.
+  apply (term_wf_forall_list_ind (fun t => forall k, wf (lift n k t))) ; simpl; intros; try constructor; auto.
+  destruct leb; constructor.
+  apply Forall_map.
+  induction H; constructor; auto.
+  now apply lift_rec_isApp.
+  now apply map_non_nil.
+  apply Forall_map. eapply Forall_impl. apply H2. auto.
+  apply Forall_map. eapply Forall_impl. apply H1.
+  intros [n' t]. simpl. repeat red; simpl; auto.
+  apply Forall_map. eapply Forall_impl. apply H.
+  simpl. intros. red; intuition (simpl; auto).
+  apply Forall_map. eapply Forall_impl. apply H.
+  simpl. intros. red; intuition (simpl; auto).
+Qed.
+
+Lemma mkApps_tApp t l :
+  ~ isApp t = true -> l <> nil -> mkApps t l = tApp t l.
+Proof.
+  intros.
+  destruct l. simpl. contradiction.
+  destruct t; simpl; try reflexivity.
+  simpl in H. contradiction.
+Qed.
+
+Hint Unfold compose.
+Hint Transparent compose.
+
+Lemma simpl_subst_rec :
+  forall M (H : wf M) N n p k,
+    p <= n + k ->
+    k <= p -> subst_rec N (lift_rec (S n) M k) p = lift_rec n M k.
+Proof.
+  intros M wfM. induction wfM using term_wf_forall_list_ind;
+    intros; simpl; try easy;
+      rewrite ?map_map_compose, ?compose_on_snd, ?compose_map_def;
+      try solve [f_equal; easy];
+      try (f_equal; try easy; apply_spec); intros;
+        try rewrite ?map_length; try easy ||
+      (try rewrite H, H0; f_equal; try easy; now f_equal).
+  
+  - elim (leb_spec k n); intros; try easy.
+    + rewrite subst_rel_gt; try easy.
+    + rewrite subst_rel_lt; try easy.
+
+  - rewrite IHwfM; auto.
+    apply (lift_rec_isApp n k) in H.
+    rewrite mkApps_tApp; auto using map_non_nil.
+    f_equal. eapply forall_map_spec. apply H1; simpl; auto.
+    simpl; intros. typeclasses eauto with core.
+Qed.
+
+Lemma simpl_subst :
+  forall N M (H : wf M) n p, p <= n -> subst_rec N (lift0 (S n) M) p = lift0 n M.
+  intros; now apply simpl_subst_rec.
+Qed.
+
+Lemma mkApps_tRel n a l : mkApps (tRel n) (a :: l) = tApp (tRel n) (a :: l).
+Proof.
+  simpl. reflexivity.
+Qed.
+
+Lemma lift_mkApps n k t l : lift n k (mkApps t l) = mkApps (lift n k t) (map (lift n k) l).
+Proof.
+  revert n k t; induction l; intros n k t; destruct t; try reflexivity.
+  rewrite lift_rel_alt. rewrite !mkApps_tRel.
+  simpl lift.
+  simpl map. rewrite !mkApps_tRel.
+  f_equal. destruct leb; auto.
+
+  simpl. f_equal.
+  now rewrite map_app.
+Qed.
+
+Lemma commut_lift_subst_rec :
+  forall M N n p k,
+    k <= p ->
+    lift_rec n (subst_rec N M p) k = subst_rec N (lift_rec n M k) (n + p).
+Proof.
+  intros M.
+  elim M using term_forall_list_ind;
+    intros; simpl; try easy;
+      rewrite ?map_map_compose, ?compose_on_snd, ?compose_map_def;
+      try solve [f_equal; easy];
+      try (f_equal; try easy; apply_spec);
+      unfold compose; intros;
+        try rewrite ?map_length; try easy ;
+        try (rewrite H, H0; f_equal; try easy; now f_equal);
+        try (rewrite H, H0, H1; f_equal; try easy; now f_equal);
+        try (rewrite H1; now f_equal).
+  
+  - elim (compare_spec p n); elim (leb_spec k n); intros; subst; try easy.
+    + rewrite subst_rel_eq; try easy.
+      now rewrite simpl_lift_rec.
+    + rewrite subst_rel_gt; try easy.
+      now rewrite lift_rel_ge.
+    + rewrite lift_rel_ge; try easy.
+      now rewrite subst_rel_lt.
+    + rewrite lift_rel_lt; try easy.
+      now rewrite subst_rel_lt.
+
+  - rewrite lift_mkApps. f_equal. auto.
+    rewrite map_map_compose. apply_spec. intros.
+    now apply H2.
+Qed.
+
+Lemma commut_lift_subst :
+  forall M N k, subst_rec N (lift0 1 M) (S k) = lift0 1 (subst_rec N M k).
+  now intros; rewrite commut_lift_subst_rec.
+Qed.
+
+Lemma distr_lift_subst_rec :
+  forall M N n p k,
+    lift_rec n (subst_rec N M p) (p + k) =
+    subst_rec (lift_rec n N k) (lift_rec n M (S (p + k))) p.
+Proof.
+  intros M.
+  elim M using term_forall_list_ind;
+    intros; match goal with
+              |- context [tRel _] => idtac
+            | |- _ => simpl
+            end; try easy;
+      rewrite ?map_map_compose, ?compose_on_snd, ?compose_map_def;
+      try solve [f_equal; easy];
+      try (f_equal; try easy; apply_spec);
+      unfold compose; intros;
+        try rewrite ?map_length; try easy ;
+        try (erewrite H, <- H0; f_equal; try easy; now f_equal);
+        try (erewrite H, <- H0, <- H1; f_equal; try easy; now f_equal);
+        try (erewrite H1; now f_equal).
+  
+  - unfold subst at 1. unfold lift at 4.
+    elim (compare_spec p n); intros; try easy;
+    elim (leb_spec (S (p + k)) n); intros; subst; try easy.
+    
+    + rewrite subst_rel_eq. now rewrite <- permute_lift_rec. 
+    + rewrite lift_rel_ge; try easy.
+      now rewrite subst_rel_gt.
+    + rewrite lift_rel_lt; try easy.
+      now rewrite subst_rel_gt.
+    + rewrite lift_rel_lt; try easy.
+      now rewrite subst_rel_lt.
+
+  - rewrite lift_mkApps. f_equal; auto.
+    rewrite map_map_compose; apply_spec; simpl.
+    intros. apply H1.
+  - rewrite add_assoc, H0. f_equal. now f_equal.
+  - rewrite add_assoc, H0. f_equal. now f_equal.
+Qed.
+
+Lemma distr_lift_subst :
+  forall M N n k,
+    lift_rec n (subst0 N M) k = subst0 (lift_rec n N k) (lift_rec n M (S k)).
+Proof.
+  intros; unfold subst in |- *.
+  pattern k at 1 3 in |- *.
+  replace k with (0 + k); try easy.
+  apply distr_lift_subst_rec.
+Qed.
+
+Lemma mkApp_nested f l l' : mkApps (mkApps f l) l' = mkApps f (l ++ l').
+Proof.
+  induction l; destruct f; destruct l'; simpl; rewrite ?app_nil_r; auto.
+  f_equal. now rewrite <- app_assoc.
+Qed.
+
+Lemma subst_mkApps u k t l : subst u k (mkApps t l) = mkApps (subst u k t) (map (subst u k) l).
+Proof.
+  revert u k t; induction l; intros u k t; destruct t; try reflexivity.
+  intros. simpl mkApps at 1. simpl subst at 2. simpl subst at 1.
+  rewrite map_app. now rewrite mkApp_nested.
+Qed.
+
+Lemma distr_subst_rec :
+  forall M N (P : term) (wfP : wf P) n p,
+    subst_rec P (subst_rec N M p) (p + n) =
+    subst_rec (subst_rec P N n) (subst_rec P M (S (p + n))) p.
+Proof.
+  intros M.
+  elim M using term_forall_list_ind;
+    intros; match goal with
+              |- context [tRel _] => idtac
+            | |- _ => simpl
+            end; try easy;
+      rewrite ?map_map_compose, ?compose_on_snd, ?compose_map_def;
+      try solve [f_equal; easy];
+      try (f_equal; try easy; apply_spec);
+      unfold compose; intros;
+        try rewrite ?map_length; try easy ;
+        try (erewrite H, <- H0; f_equal; try easy; now f_equal);
+        try (erewrite H, <- H0, <- H1; f_equal; try easy; now f_equal);
+        try (erewrite H1; now f_equal).
+  
+  - unfold subst at 2. 
+    elim (compare_spec p n); intros; try easy.
+    
+    + subst. rewrite subst_rel_lt; try easy.
+      rewrite subst_rel_eq; try easy.
+      now rewrite <- commut_lift_subst_rec.
+    + unfold subst at 4.
+      elim (compare_spec (S (p + n0)) n); intros; subst; try easy.
+      ++ rewrite subst_rel_eq.
+         now rewrite simpl_subst_rec.
+      ++ rewrite !subst_rel_gt; try easy.
+      ++ rewrite subst_rel_lt; try easy.
+         now rewrite subst_rel_gt.
+    + rewrite !subst_rel_lt; try easy.
+
+  - rewrite !subst_mkApps. rewrite H; auto. f_equal.
+    rewrite !map_map_compose. apply_spec. intros.
+    unfold compose. auto.
+  - rewrite add_assoc, H0; auto. f_equal. now f_equal.
+  - rewrite add_assoc, H0; auto. f_equal. now f_equal.
+Qed.
+
+Lemma distr_subst :
+  forall (P : term) (wfP : wf P) N M k,
+    subst_rec P (subst0 N M) k = subst0 (subst_rec P N k) (subst_rec P M (S k)).
+Proof.
+  intros; unfold subst in |- *.
+  pattern k at 1 3 in |- *.
+  change k with (0 + k).
+  now apply distr_subst_rec.
+Qed.
+
+
+Lemma lift_closed n k t : closedn k t = true -> lift n k t = t.
+Proof.
+  revert k.
+  elim t using term_forall_list_ind; intros; try easy;
+    rewrite ?map_map_compose, ?compose_on_snd, ?compose_map_def;
+    try (f_equal; apply_spec);  simpl closed in *;
+    try rewrite ?map_length; try easy.
+  - rewrite lift_rel_lt; auto.
+    revert H. elim (Nat.ltb_spec n0 k); intros; try easy.
+  - simpl lift; f_equal.
+    rewrite <- map_id. 
+    apply_spec; eauto.
+  - simpl lift. rewrite andb_true_iff in H1. f_equal; intuition eauto.
+  - simpl lift; rewrite andb_true_iff in H1. f_equal; intuition eauto.
+  - simpl lift. rewrite !andb_true_iff in H2. f_equal; intuition eauto.
+  - simpl lift. rewrite !andb_true_iff in H1. f_equal; intuition eauto.
+    rewrite <- map_id; apply_spec; eauto.
+  - simpl lift. rewrite !andb_true_iff in H2. f_equal; intuition eauto.
+    transitivity (map (on_snd id) l). apply_spec; eauto.
+    rewrite <- map_id. f_equal. unfold on_snd. extensionality p. now destruct p.
+  - simpl lift. f_equal; eauto.
+  - simpl lift. f_equal.
+    transitivity (map (map_def id) m). apply_spec; eauto.
+    now autorewrite with core.
+  - simpl lift. f_equal.
+    transitivity (map (map_def id) m). apply_spec; eauto.
+    now autorewrite with core.
+Qed.
