template-coq/theories/Retyping.v
@@ -1,12 +1,14 @@
 (* Distributed under the terms of the MIT license.   *)
 
 From Coq Require Import Bool String List Program BinPos Compare_dec Omega.
-From Template Require Import Template monad_utils utils Ast univ Induction LiftSubst UnivSubst Typing Checker.
+From Template Require Import config monad_utils utils Ast univ Induction LiftSubst UnivSubst Typing Checker.
 From Template Require AstUtils.
 Require Import String.
 Local Open Scope string_scope.
 Set Asymmetric Patterns.
 Import monad_utils.MonadNotation.
+
+Existing Instance default_checker_flags.
 
 (** * Retyping
 
